src/robot.lean
@@ -16,22 +16,27 @@ section
         |n (h :: t) := (f n h) :: (mapi_aux (nat.succ n) t)
         def list.mapi (f : ℕ → α → β) := mapi_aux f 0
     end
+    section
     variables {m : Type → Type} [applicative m] {α : Type} -- [HACK] I got bored trying to get the universe poly to work.
-    def list.filterm (pred : α → m (bool)) : list α → m (list α)
-    |[] := pure []
-    |(h::t) := pure (λ (b:bool) t, if b then h::t else t) <*> pred h <*> list.filterm t
-    def list.anym (pred : α → m bool) : list α → m bool
-    |[] := pure ff
-    |(h::t) := pure bor <*> pred h <*> list.anym t
-    def list.allm (pred : α → m bool) : list α → m bool
-    |[] := pure tt
-    |(h::t) := pure band <*> pred h <*> list.allm t
+        def list.filterm (pred : α → m (bool)) : list α → m (list α)
+        |[] := pure []
+        |(h::t) := pure (λ (b:bool) t, if b then h::t else t) <*> pred h <*> list.filterm t
+    end
+    section
+        variables {m : Type → Type} [monad m] {α : Type}
+        def list.anym (pred : α → m bool) : list α → m bool
+        |[] := pure ff
+        |(h::t) := do b ← pred h, if b then pure tt else list.anym t
+        def list.allm (pred : α → m bool) : list α → m bool
+        |[] := pure tt
+        |(h::t) := do b ← pred h, if b then list.allm t else pure ff
+    end
 end 
 
 /--Run the given tactic, get the returned value. But don't keep the tactic's state. -/
 meta def tactic.hypothetically {α} (tb : tactic α) : tactic α :=
     λ s, result.cases_on (tb s)
-        (λ a s, interaction_monad.result.success a s)
+        (λ a _, interaction_monad.result.success a s)
         interaction_monad.result.exception
 
 /--This information is needed so frequently I'm bundling them into their own structure.-/
@@ -40,10 +45,13 @@ meta structure statement :=
 (type : expr)
 (refs : table expr)
 
+meta instance : has_to_tactic_format statement := ⟨λ a, do bpp ← tactic.pp a.body, tpp ← tactic.pp a.type, pure $ bpp ++ " : " ++ tpp⟩
+
 /--Robot needs some extra data on hypotheses to track when things can be deleted and so on.-/
 meta structure hyp_datum :=
 (vuln : bool) -- the hypothesis has been used previously and so is vulnerable for deletion.
 (cannot_substitute : dict nat (table expr)) -- The expressions that have previously been used on the nth argument.
+meta def hyp_datum.init : hyp_datum := {vuln := ff , cannot_substitute := empty}
 
 @[reducible] meta def hyp_data := dict expr hyp_datum
 
@@ -69,6 +77,9 @@ namespace robot
         hd ← get_hyp_data,
         cs ← list.filter (λ x, show bool, from option.cases_on (get x hd) ff hyp_datum.vuln) <$> tactic.local_context,
         list.choosem get_statement cs
+    meta def set_vuln (h : expr) : robot unit :=
+        -- [TODO] make sure it really is a hypothesis and not just some random expression.
+        map_hyp_data (dict.modify_default hyp_datum.init (λ hd, {vuln := tt, ..hd}) h)
     meta def get_cannot_substitute (hyp:expr) : robot (dict nat (table expr)) := do
         hd ←  dict.get hyp <$> get_hyp_data,
         pure $ option.get_or_else (hyp_datum.cannot_substitute <$> hd) empty
@@ -78,8 +89,22 @@ namespace robot
     meta def clear_hyp (h : expr) : robot unit := do
         tactic.clear h,
         map_hyp_data (dict.erase h)
-    /--Run given tactic. But throw away the state made by the tactic.-/
+    /--Run the given tactic. But throw away the state made by the tactic.-/
     meta def hypothetically {α} (t : robot α) : robot α :=
         ⟨λ rs, tactic.hypothetically (t.run rs)⟩
-
+    meta def init : tactic (robot_state) := pure {hyp_data := empty}
+    meta def run {α} (r : robot α) : (tactic α) := do
+        i ← init,
+        ⟨a,s⟩ ← state_t.run r i,
+        pure a
 end robot
+
+section TEST
+--test `hypothetically`
+variables (p q r : Prop)
+example : p → q → q := begin
+    intros,
+    tactic.hypothetically (do tactic.set_goals []),
+    assumption
+end
+end TEST
